theories/Core/Semantic/PER.v
@@ -1,1 +1,1 @@
-From Mcltt Require Export PER.Definitions PER.Lemmas.
+From Mcltt Require Export PER.Definitions PER.Lemmas PER.CoreTactics.
